---
title: "Demostración alternativa de la varianza"
author: "Téllez Gerardo Rubén"
date: "20/12/2021"
output: ioslides_presentation
---

```{r setup, include=FALSE}
knitr::opts_chunk$set(echo = FALSE)
```

## Formulas

$$\sigma^2 = \frac{\sum{(x_i - \bar{x})^2}}{m}$$

$$\sigma^2 = \frac{\sum{(x_i)^2}}{m} - \bar{x}^2$$

$$m \cdot \sigma^2 = \sum{(x_i} - \bar{x})^2$$

## Formulas

$$m \cdot \sigma^2 = \sum{(x_i} - \bar{x})^2 = \sum{(x_i}^2 - 2x_i\bar{x} + \bar{x}^2)$$

$$\sum x_i^2 - 2 \sum x_i\bar{x} + \sum \bar{x}^2$$

$$\sum x_i^2 - 2\bar{x} \sum x_i + m\bar{x}^2$$

## Formulas


$$\bar{x} = \frac{\sum x_i}{m}$$

$$\sum x_i^2 - 2\bar{x}\cdot m \bar{x} + m \bar{x}^2$$

$$\sum x_i^2 - 2m\bar{x}^2 + m\bar{x}^2$$

## Formulas


$$\sum x_i^2 - m\bar{x}^2$$

$$m \sigma^2 = \sum x_i^2 - m\bar{x}^2$$

$$\sigma^2 = \frac{\sum x_i^2}{m} - \bar{x}^2$$


